unfinished work on descendents

DFS.v
@@ -1340,6 +1340,157 @@ Proof.
       apply IHl1.
 Qed. 
 
+(*The descedant of a vertex (in terms of the stack). We will prove that it is equivalent
+  to being a descendent in the DFS forest*)
+Inductive stack_desc: state -> vertex -> vertex -> Prop :=
+  | parent: forall x y s, In (x, Some y) (get_stack s) -> stack_desc s x y
+  | path: forall x y z s, stack_desc s x y -> In (y, Some z) (get_stack s) -> stack_desc s x z.
+
+Lemma stack_desc_trans: forall x y z s,
+  stack_desc s x y ->
+  stack_desc s y z ->
+  stack_desc s x z.
+Proof.
+  intros. induction H0.
+  - eapply path. apply H. apply H0.
+  - eapply path. apply IHstack_desc. apply H. apply H1.
+Qed.
+
+Lemma stack_desc_has_child: forall x y s,
+  stack_desc s x y -> 
+  In (x, Some y) (get_stack s) \/ exists z, stack_desc s x z /\ In (z, Some y) (get_stack s).
+Proof.
+  intros. induction H.
+  - left. apply H.
+  - destruct IHstack_desc. right. exists y. split. apply H. apply H0.
+    destruct H1. destruct H1. right. exists y. split. apply H. apply H0.
+Qed. 
+
+Lemma stack_desc_has_child_rev: forall x y s,
+  stack_desc s x y -> 
+  In (x, Some y) (get_stack s) \/ exists z,  In (x, Some z) (get_stack s) /\ stack_desc s z y.
+Proof.
+  intros. induction H.
+  - left. apply H.
+  - destruct IHstack_desc. right. exists y. split. apply H1. eapply parent. apply H0. 
+    destruct H1. destruct H1. right. exists x0. split. apply H1. eapply stack_desc_trans.
+    apply H2. apply parent. apply H0.  
+Qed. 
+
+
+
+
+(*
+Lemma right_left_stacks: forall s g o v,
+  valid_dfs_state s g o ->
+  exists tl o',
+  gray s v = true ->
+  (exists l1, get_stack s = l1 ++ (v,o') :: tl /\ (forall o'', ~In (v, o'') l1) /\
+  (forall y, ~In (y, Some v) tl) /\ (forall x, stack_desc s x v <-> exists p, In (x,p) l1)).
+Proof.
+  intros. unfold gray in *. induction H; subst; simpl in *.
+  - destruct o. destruct (G.contains_vertex g v0) eqn : ?.
+    + exists nil. exists None. intros. simplify. rewrite H1 in H0. inversion H0.
+    + exists nil. exists None. intros. simplify. rewrite H1 in H0. inversion H0.
+    + exists nil. exists None. intros. simplify. rewrite H1 in H0. inversion H0.
+  - inversion H0; subst; simpl in *; destruct IHvalid_dfs_state.
+    + destruct H3. assert (tl = nil). eapply root_nil. eapply step. apply H. apply H0. simpl. reflexivity.
+    subst. destruct (O.eq_dec x v). 
+      * unfold O.eq in e. subst. exists nil. exists None. intros. exists (add_to_stack v g0 remain_d).
+        split. reflexivity. intros. split. intros. intro. apply add_to_stack_neq in H5. contradiction.
+        split. intros. intro. inversion H5. intros; split; intros. apply stack_desc_has_child in H5; simpl in *.
+        destruct H5. exists (Some v). apply in_app_or in H5. destruct H5. apply H5. simpl in H5.
+        destruct H5; inversion H5. destruct H5. destruct H5. apply stack_desc_has_child in H5; simpl in *.
+        destruct H5. apply in_app_or in H5. destruct H5. apply add_to_stack_adds_parent in H5.
+        inversion H5; subst. exfalso. eapply neq_parent. eapply step. apply H. apply H0. simpl.
+        apply H6. reflexivity. simpl in H5. destruct H5; inversion H5. destruct H5. destruct H5.
+        apply in_app_or in H7. destruct H7. apply add_to_stack_adds_parent in H7. inversion H7; subst.
+        exfalso. eapply neq_parent. eapply step. apply H. apply H0. simpl. apply H6. reflexivity.
+        destruct H7; inversion H7. destruct H5. eapply parent. simpl. 
+        assert (x2 = Some v). eapply add_to_stack_adds_parent. apply H5. subst. apply in_or_app.
+        left. apply H5. 
+      * (*doesn't matter, this is impossible*)
+        exists nil. exists None. intros. remember (g0, f, f_times, d_times, time, remain_d, remain_f, st) as s.
+       assert (exists o, In (v, o) (get_stack s)). eapply gray_on_stack. apply H.
+       unfold gray; subst; simpl in *. simplify. rewrite P2.FM.remove_neq_b in H5. apply H5. intuition.
+       subst; simpl in *. destruct H5. destruct (pop_stack st remain_f) eqn : ?.
+       -- simpl in H2. rewrite pop_stack_nil in Heqs. specialize (Heqs (v, x2)).
+          simpl in Heqs. apply Heqs in H5. simplify. rewrite H5 in H7. inversion H7.
+       -- simpl in H2. inversion H2; subst. eapply (pop_stack_delete _ remain_f) in H5.
+          destruct H5. simplify. rewrite H7 in H5. inversion H5.
+          rewrite Heqs in H5. simpl in H5. destruct H5. inversion H5. subst. simplify. exfalso. apply n.
+          reflexivity. destruct H5.
+    + destruct H3. destruct (O.eq_dec x v).
+      * exists tl. exists (Some y). intros. exists (add_to_stack x g0 remain_d). split. 
+        rewrite e. reflexivity. assert (forall o'' : option O.t, ~ In (v, o'') (add_to_stack x g0 remain_d)).
+        intros. intro. apply add_to_stack_neq in H5. rewrite e in H5.
+        contradiction. split. apply H5. assert (forall y0, ~In (y0, Some v) tl). intros.
+        intro. rewrite e in H1. 
+        remember (g0, t :: f, f_times, d_times, time, remain_d, remain_f, st) as s.
+        assert (white s v = true). unfold white; subst; simpl; simplify.
+        pose proof parents_not_white. specialize (H8 s g o y0 v). apply H8 in H. rewrite H in H7. inversion H7.
+         subst; simpl. destruct (pop_stack st remain_f) eqn : ?.
+        -- simpl in H2. destruct (S.min_elt remain_d). inversion H2; subst. inversion H2.
+        -- simpl in H2. rewrite <- H2 in Heqs. eapply in_pop_rev. rewrite Heqs. right. apply H6.
+        -- split. apply H6. intros; split; intros.
+          ++ apply stack_desc_has_child in H7; simpl in H7. destruct H7.
+             apply in_app_or in H7. destruct H7. exists (Some v). apply H7.
+             simpl in H7. destruct H7. inversion H7; subst. rewrite e in H2.
+             exfalso. eapply neq_parent. eapply step. apply H. apply H0. simpl. apply in_or_app.
+             right. left. reflexivity. apply e. specialize (H6 x2). contradiction.
+             destruct H7. destruct H7. apply stack_desc_has_child in H7; simpl in H7. destruct H7.
+             apply in_app_or in H8. destruct H8. assert (B:=H8). apply add_to_stack_adds_parent in H8. inversion H8; subst.
+             apply in_app_or in H7. destruct H7. assert (A:=H7). apply add_to_stack_adds_parent in H7. inversion H7; subst.
+             exists (Some x). apply A. assert (C:= H7). simpl in H7. destruct H7. inversion H7; subst.
+             Search add_to_stack.
+             
+             
+             
+             
+
+
+ destruct H6. apply add_to_stack_adds_parent in H6.  inversion H6; subst.
+             exfalso. eapply neq_parent. eapply step. apply H. apply H0. simpl. apply H7. apply e.
+             apply in_app_or in H7. destruct H7. exfalso. eapply neq_parent. eapply step. apply H. apply H0.
+              simpl. apply in_or_app. left. apply H7. apply add_to_stack_adds_parent in H7. inversion H7.
+
+             apply in_app_or in H7. destruct H7. apply add_to_stack_adds_parent in H7. inversion H7; subst.
+             
+             
+      * exists x0. exists x1. intros. destruct H3.
+        rewrite P2.FM.remove_neq_b in H4. apply H4. apply n.
+        destruct (pop_stack st) eqn : ?.
+        -- simpl in H2. destruct (S.min_elt remain_d); inversion H2.
+        -- simpl in H2. exists (add_to_stack x g0 remain_d ++ (pop_stack (x2) remain_f)).
+        split. destruct H3. rewrite H2. rewrite <- Heqs. rewrite H3. rewrite pop_stack_app_distr.
+        rewrite app_assoc. reflexivity. simplify. split. intros. intro. apply in_app_or in H5.
+        destruct H5. apply only_add_yet_to_be_discovered in H5. simplify.
+        rewrite P2.FM.remove_neq_b in H6. rewrite H6 in H5. inversion H5. intuition. 
+        destruct H3. destruct H6. apply (H6 o''). eapply in_pop_rev. apply H5.
+        intros. intro. destruct H3. destruct H6. apply (H7 y0). apply H5.
+    + destruct H4. destruct (O.eq_dec x v).
+      * unfold O.eq in e. subst. destruct H4. simplify. destruct H4.
+        exists x0. exists x1. intros. simplify. exfalso. eapply remove_eq. apply H9.
+      * exists x0. exists x1. intros. simplify.
+        rewrite P2.FM.remove_neq_b in H7. destruct H4. assumption.
+        destruct (pop_stack st remain_f) eqn : ?.
+        -- simpl in H3. destruct (S.min_elt remain_d) eqn : ?; inversion H3; subst.
+           remember (g0, f, M.add e (time + 1) f_times, d_times, time + 1, remain_d, S.remove e remain_f, nil) as s.
+           assert (exists o, In (v,o) (get_stack s)). eapply gray_on_stack. eapply step. apply H.
+           apply H0. unfold gray. subst; simpl; simplify. subst; simpl in *. destruct H5. destruct H5.
+        -- simpl in H3. rewrite <- H3 in Heqs.
+            destruct H4. rewrite H4 in Heqs. rewrite pop_stack_app_distr in Heqs.
+            destruct (pop_stack x2 remain_f) eqn : ?.
+            ++ inversion Heqs; subst. exfalso. apply n. reflexivity.
+            ++ inversion Heqs; subst. exists s0. split. reflexivity. split. intros.
+               destruct H5.
+               apply (H5 o''). eapply in_pop_rev. rewrite Heqs0. right. apply H4.
+                destruct H5. apply H5.
+            ++ apply H7.
+       -- intuition.
+Qed. 
+*)
+
 (*An important lemma: The stack to the left of a gray vertex does not change. Moreover,
   the rest of the stack does not contain v, and the previous does not have v as a parent.
   This is key to proving that the search proceeds in a depth first manner*)
@@ -1415,6 +1566,8 @@ Proof.
             ++ apply H7.
        -- intuition.
 Qed. 
+
+
 
 
 (*
@@ -1505,6 +1658,248 @@ Lemma parent_gray_when_child_active: forall s g o x y,
 Proof.
   intros. eapply parent_gray. apply H. exists x. apply H0.
 Qed.
+
+Lemma stack_desc_child: forall x y s,
+  stack_desc s x y -> (exists z, In (z, Some y) (get_stack s)).
+Proof.
+  intros. induction H.
+  - exists x. apply H.
+  - exists y. apply H0.
+Qed.
+
+Lemma stack_desc_child_first: forall x y s,
+  stack_desc s x y -> (exists z, In (x, Some z) (get_stack s)).
+Proof.
+  intros. induction H.
+  - exists y. apply H.
+  - destruct IHstack_desc. exists x0. apply H1.
+Qed.
+
+Lemma right_left_stacks': forall s g o v,
+  valid_dfs_state s g o ->
+  exists tl o',
+  gray s v = true ->
+  (exists l1, get_stack s = l1 ++ (v,o') :: tl /\ (forall o'', ~In (v, o'') l1) /\
+  (forall y, ~In (y, Some v) tl) /\ (forall x, stack_desc s x v <-> exists p, In (x,p) l1)).
+Proof.
+  intros. unfold gray in *. induction H; subst; simpl in *.
+  - destruct o. destruct (G.contains_vertex g v0) eqn : ?.
+    + exists nil. exists None. intros. simplify. rewrite H1 in H0. inversion H0.
+    + exists nil. exists None. intros. simplify. rewrite H1 in H0. inversion H0.
+    + exists nil. exists None. intros. simplify. rewrite H1 in H0. inversion H0.
+  - inversion H0; subst; simpl in *; destruct IHvalid_dfs_state.
+    + destruct H3. assert (tl = nil). eapply root_nil. eapply step. apply H. apply H0. simpl. reflexivity.
+    subst. destruct (O.eq_dec x v). 
+      * unfold O.eq in e. subst. exists nil. exists None. intros. exists (add_to_stack v g0 remain_d).
+        split. reflexivity. intros. split. intros. intro. apply add_to_stack_neq in H5. contradiction.
+        split. intros. intro. inversion H5. intros; split; intros. apply stack_desc_has_child in H5; simpl in *.
+        destruct H5. exists (Some v). apply in_app_or in H5. destruct H5. apply H5. simpl in H5.
+        destruct H5; inversion H5. destruct H5. destruct H5. apply stack_desc_has_child in H5; simpl in *.
+        destruct H5. apply in_app_or in H5. destruct H5. apply add_to_stack_adds_parent in H5.
+        inversion H5; subst. exfalso. eapply neq_parent. eapply step. apply H. apply H0. simpl.
+        apply H6. reflexivity. simpl in H5. destruct H5; inversion H5. destruct H5. destruct H5.
+        apply in_app_or in H7. destruct H7. apply add_to_stack_adds_parent in H7. inversion H7; subst.
+        exfalso. eapply neq_parent. eapply step. apply H. apply H0. simpl. apply H6. reflexivity.
+        destruct H7; inversion H7. destruct H5. eapply parent. simpl. 
+        assert (x2 = Some v). eapply add_to_stack_adds_parent. apply H5. subst. apply in_or_app.
+        left. apply H5. 
+      * (*doesn't matter, this is impossible*)
+        exists nil. exists None. intros. remember (g0, f, f_times, d_times, time, remain_d, remain_f, st) as s.
+       assert (exists o, In (v, o) (get_stack s)). eapply gray_on_stack. apply H.
+       unfold gray; subst; simpl in *. simplify. rewrite P2.FM.remove_neq_b in H5. apply H5. intuition.
+       subst; simpl in *. destruct H5. destruct (pop_stack st remain_f) eqn : ?.
+       -- simpl in H2. rewrite pop_stack_nil in Heqs. specialize (Heqs (v, x2)).
+          simpl in Heqs. apply Heqs in H5. simplify. rewrite H5 in H7. inversion H7.
+       -- simpl in H2. inversion H2; subst. eapply (pop_stack_delete _ remain_f) in H5.
+          destruct H5. simplify. rewrite H7 in H5. inversion H5.
+          rewrite Heqs in H5. simpl in H5. destruct H5. inversion H5. subst. simplify. exfalso. apply n.
+          reflexivity. destruct H5.
+    + destruct H3. destruct (O.eq_dec x v).
+      * exists tl. exists (Some y). intros. exists (add_to_stack x g0 remain_d). split. 
+        rewrite e. reflexivity. assert (forall o'' : option O.t, ~ In (v, o'') (add_to_stack x g0 remain_d)).
+        intros. intro. apply add_to_stack_neq in H5. rewrite e in H5.
+        contradiction. split. apply H5. assert (forall y0, ~In (y0, Some v) tl). intros.
+        intro. rewrite e in H1. 
+        remember (g0, t :: f, f_times, d_times, time, remain_d, remain_f, st) as s.
+        assert (white s v = true). unfold white; subst; simpl; simplify.
+        pose proof parents_not_white. specialize (H8 s g o y0 v). apply H8 in H. rewrite H in H7. inversion H7.
+         subst; simpl. destruct (pop_stack st remain_f) eqn : ?.
+        -- simpl in H2. destruct (S.min_elt remain_d). inversion H2; subst. inversion H2.
+        -- simpl in H2. rewrite <- H2 in Heqs. eapply in_pop_rev. rewrite Heqs. right. apply H6.
+        -- split. apply H6. intros; split; intros.
+          ++ apply stack_desc_has_child in H7; simpl in H7. destruct H7.
+             apply in_app_or in H7. destruct H7. exists (Some v). apply H7.
+             simpl in H7. destruct H7. inversion H7; subst. rewrite e in H2.
+             exfalso. eapply neq_parent. eapply step. apply H. apply H0. simpl. apply in_or_app.
+             right. left. reflexivity. apply e. specialize (H6 x2). contradiction.
+             destruct H7. destruct H7. apply stack_desc_child in H7. destruct H7; simpl in *.
+             apply in_app_or in H8. destruct H8. assert (B:=H8). apply add_to_stack_adds_parent in H8. inversion H8; subst.
+             apply in_app_or in H7. destruct H7. assert (A:=H7). apply add_to_stack_adds_parent in H7. inversion H7; subst.
+             exfalso. eapply neq_parent. eapply step. apply H. apply H0. simpl. apply in_or_app.
+              left. apply B. reflexivity.
+             remember (g0, T.add_child t y x :: f, f_times, M.add x (time + 1) d_times, time + 1, S.remove x remain_d, remain_f,
+       add_to_stack x g0 remain_d ++ (x, Some y) :: tl) as s.
+             assert (gray s x3 = true). eapply parent_gray. eapply step. apply H. subst. apply H0.
+              subst. simpl. exists x4. apply in_or_app. right. apply H7. 
+              assert (B':=B). apply only_add_yet_to_be_discovered in B.
+              apply add_to_stack_neq in B'. unfold gray in H9. subst; simpl in *.
+              rewrite andb_true_iff in H9. destruct H9. rewrite P2.FM.remove_neq_b in H9.
+              rewrite B in H9. inversion H9. intuition. simpl in H8. destruct H8.
+              inversion H8; subst. unfold O.eq in e. subst. exfalso. eapply neq_parent.
+              eapply step. apply H. apply H0. simpl. apply in_or_app. right. left. reflexivity.
+              reflexivity. specialize (H6 x3). contradiction.
+            ++ eapply parent. simpl. destruct H7. apply in_or_app. left.
+               assert (A:=H7). apply add_to_stack_adds_parent in H7. subst. rewrite <- e. apply A.  
+      * exists x0. exists x1. intros. destruct H3.
+        rewrite P2.FM.remove_neq_b in H4. apply H4. apply n.
+        destruct (pop_stack st) eqn : ?.
+        -- simpl in H2. destruct (S.min_elt remain_d); inversion H2.
+        -- simpl in H2. exists (add_to_stack x g0 remain_d ++ (pop_stack (x2) remain_f)).
+        split. destruct H3. rewrite H2. rewrite <- Heqs. rewrite H3. rewrite pop_stack_app_distr.
+        rewrite app_assoc. reflexivity. simplify.
+        assert (forall o'' : option O.t, ~ In (v, o'') (add_to_stack x g0 remain_d ++ pop_stack x2 remain_f)).
+         intros. intro. apply in_app_or in H5.
+        destruct H5. apply only_add_yet_to_be_discovered in H5. simplify.
+        rewrite P2.FM.remove_neq_b in H6. rewrite H6 in H5. inversion H5. intuition. 
+        destruct H3. destruct H6. apply (H6 o''). eapply in_pop_rev. apply H5.
+        split. apply H5. assert (forall y0 : S.elt, ~ In (y0, Some v) x0) .
+        intros. intro. destruct H3. destruct H7. destruct H8. apply (H8 y0). apply H6. split. apply H6.
+        intros. split; intros.
+        ++ apply stack_desc_has_child_rev in H7; simpl in H7; destruct H7.
+          ** destruct H3. destruct H8. destruct H9. apply in_app_or in H7. destruct H7.
+             apply add_to_stack_adds_parent in H7. inversion H7; subst. exfalso. apply n. reflexivity.
+              simpl in H7. destruct H7. inversion H7; subst.
+            rewrite pop_stack_app_distr in Heqs. rewrite <- H2 in Heqs.
+            destruct (pop_stack x2 remain_f) eqn : ?; simpl in Heqs.
+            inversion Heqs; subst. exfalso. apply n. reflexivity. inversion Heqs; subst.
+            exists (Some v). apply in_or_app. right. left. reflexivity. simplify.
+            subst. rewrite <- H2 in Heqs. rewrite pop_stack_app_distr in Heqs.
+             destruct (pop_stack (x2) remain_f) eqn : ?; simpl in Heqs. inversion Heqs; subst.
+            exfalso. apply n. reflexivity. inversion Heqs; subst. inversion H2; subst.
+            apply in_app_or in H7. destruct H7. exists (Some v). apply in_or_app. right. right.
+            apply H3. simpl in H3. destruct H3. inversion H3; subst.
+            exfalso. eapply neq_parent. eapply step. apply H. apply H0. simpl.
+            apply in_or_app. right. simpl. right. apply in_or_app. right. left. reflexivity. reflexivity.
+            specialize (H9 x3). contradiction. simplify.
+          ** destruct H7. destruct H7. apply stack_desc_child_first in H7. destruct H7; simpl in H7.
+             
+
+
+destruct H3. destruct H8. destruct H9. destruct H7. destruct H7. apply in_app_or in H11. destruct H11.
+             apply add_to_stack_adds_parent in H11. inversion H11; subst. exfalso. apply n. reflexivity.
+              simpl in H11. destruct H11. inversion H11; subst.
+            rewrite pop_stack_app_distr in Heqs. rewrite <- H2 in Heqs.
+            destruct (pop_stack x2 remain_f) eqn : ?; simpl in Heqs.
+            inversion Heqs; subst. exfalso. apply n. reflexivity. inversion Heqs; subst.
+            
+            exists (Some v). apply in_or_app. right. left. reflexivity. simplify.
+            subst. rewrite <- H2 in Heqs. rewrite pop_stack_app_distr in Heqs.
+             destruct (pop_stack (x2) remain_f) eqn : ?; simpl in Heqs. inversion Heqs; subst.
+            exfalso. apply n. reflexivity. inversion Heqs; subst. inversion H2; subst.
+            apply in_app_or in H7. destruct H7. exists (Some v). apply in_or_app. right. right.
+            apply H3. simpl in H3. destruct H3. inversion H3; subst.
+            exfalso. eapply neq_parent. eapply step. apply H. apply H0. simpl.
+            apply in_or_app. right. simpl. right. apply in_or_app. right. left. reflexivity. reflexivity.
+            specialize (H9 x3). contradiction. simplify.
+            remember (g0, T.add_child t y x :: f, f_times, M.add x (time + 1) d_times, time + 1, S.remove x remain_d, remain_f,
+       add_to_stack x g0 remain_d ++ (x, Some y) :: s0 ++ (x3, Some x3) :: x0) as s.
+            assert (gray s x3 = true). left.
+            refl 
+            inversion Heqs. inversion Heqs; subst.  right Search x2.
+    + destruct H4. destruct (O.eq_dec x v).
+      * unfold O.eq in e. subst. destruct H4. simplify. destruct H4.
+        exists x0. exists x1. intros. simplify. exfalso. eapply remove_eq. apply H9.
+      * exists x0. exists x1. intros. simplify.
+        rewrite P2.FM.remove_neq_b in H7. destruct H4. assumption.
+        destruct (pop_stack st remain_f) eqn : ?.
+        -- simpl in H3. destruct (S.min_elt remain_d) eqn : ?; inversion H3; subst.
+           remember (g0, f, M.add e (time + 1) f_times, d_times, time + 1, remain_d, S.remove e remain_f, nil) as s.
+           assert (exists o, In (v,o) (get_stack s)). eapply gray_on_stack. eapply step. apply H.
+           apply H0. unfold gray. subst; simpl; simplify. subst; simpl in *. destruct H5. destruct H5.
+        -- simpl in H3. rewrite <- H3 in Heqs.
+            destruct H4. rewrite H4 in Heqs. rewrite pop_stack_app_distr in Heqs.
+            destruct (pop_stack x2 remain_f) eqn : ?.
+            ++ inversion Heqs; subst. exfalso. apply n. reflexivity.
+            ++ inversion Heqs; subst. exists s0. split. reflexivity. split. intros.
+               destruct H5.
+               apply (H5 o''). eapply in_pop_rev. rewrite Heqs0. right. apply H4.
+                destruct H5. apply H5.
+            ++ apply H7.
+       -- intuition.
+Qed. 
+
+(*maybe come back but its a ton of repetition*)
+
+Lemma right_left_stack': forall s g o v,
+  valid_dfs_state s g o ->
+  exists tl o',
+  gray s v = true ->
+  (exists l1, get_stack s = l1 ++ (v,o') :: tl /\ (forall o'', ~In (v, o'') l1) /\
+  (forall y, ~In (y, Some v) tl) /\ (forall x, stack_desc s x v <-> exists p, In (x,p) l1)).
+Proof.
+  intros. pose proof right_left_stacks. assert (A:=H). eapply H0 in H. destruct H. destruct H. exists x. exists x0.
+  intros. assert (B:= H1). apply H in H1. destruct H1. exists x1. repeat(split; try (apply H1)).
+  clear H0. clear H. unfold gray in *. generalize dependent x1. induction A; intros; subst; simpl in *.
+  - simplify. rewrite H0 in H2. inversion H2.
+  - inversion H; subst; simpl in *.
+    + destruct H1. destruct H4. assert (tl = nil). eapply root_nil. eapply step. 
+      apply A. apply H. simpl. reflexivity. subst.
+      destruct (O.eq_dec x3 v).
+      * unfold O.eq in e. subst. destruct x. simpl in H1. eapply (app_inversion) in H1.
+        destruct H1. inversion H6; subst. 
+      apply stack_desc_has_child in H0; simpl in H0. destruct H0.
+       exists (Some v). apply in_app_or in H0. destruct H0. apply H0.
+      simpl in H0. destruct H0; inversion H0. destruct H0. destruct H0.
+      apply stack_desc_has_child in H0; simpl in H0; destruct H0.
+      apply in_app_or in H0. apply in_app_or in H1. destruct H0. 
+      apply add_to_stack_adds_parent in H0.  inversion H0; subst. exfalso.
+      eapply neq_parent. eapply step. apply A. apply H. simpl. apply in_or_app. apply H1. reflexivity.
+      destruct H0; inversion H0. destruct H0. destruct H0. 
+      apply in_app_or in H7. destruct H7.
+      apply add_to_stack_adds_parent in H7. inversion H7; subst. exfalso. eapply neq_parent.
+      eapply step. apply A. apply H. simpl. apply H1. reflexivity. destruct H7; inversion H7.
+      pose proof (app_inversion_2). specialize (H6 _ (v, None) (add_to_stack v g0 remain_d)
+      (x1 ++ (v, x0) :: nil) (p :: x)). destruct H6. intro. inversion H6.
+      rewrite <- app_assoc. symmetry. apply H1. rewrite H6 in H1.
+      pose proof app_inversion. specialize (H7 _ (v, None) (v, None) (add_to_stack v g0 remain_d)
+      (x1 ++ (v, x0) :: x3)). destruct H7. rewrite <- app_assoc. apply H1. 
+      exfalso. eapply neq_parent. eapply step. apply A. apply H. simpl. rewrite H7. apply in_or_app.
+      left. apply in_or_app. right. left. assert (In (v, x0) (add_to_stack v g0 remain_d)).
+      rewrite H7. apply in_or_app. right. left. reflexivity. apply add_to_stack_adds_parent in H9.
+      rewrite H9. reflexivity.  reflexivity.
+      * destruct x. apply app_inversion in H1. destruct H1. inversion H6; subst. exfalso.
+        apply n. reflexivity. pose proof (app_inversion_2 _ (x3, None) (add_to_stack x3 g0 remain_d)
+        (x1 ++ (v, x0) :: nil) (p :: x)). destruct H6. intro. inversion H6.
+        rewrite <- app_assoc. symmetry. apply H1. rewrite H6 in H1.
+        pose proof (app_inversion _ (x3, None) (x3, None) (add_to_stack x3 g0 remain_d) (x1 ++ (v, x0) :: x4)).
+        destruct H7. rewrite <- app_assoc. apply H1. assert (In (v, x0) (add_to_stack x3 g0 remain_d)).
+        rewrite H7. apply in_or_app. right. left. reflexivity. assert (A1:=H9). apply add_to_stack_adds_parent
+        in H9. subst. apply stack_desc_has_child in H0; simpl in H0. destruct H0.
+        apply in_app_or in H0. destruct H0. apply add_to_stack_adds_parent in H0. inversion H0. subst.
+        exfalso. apply n. reflexivity. destruct H0; inversion H0.
+        destruct H0. destruct H0. apply in_app_or in H9. destruct H9. apply add_to_stack_adds_parent in H9.
+        inversion H9; subst. exfalso. apply n. reflexivity. destruct H9; inversion H9.
+    + destruct H1. destruct H4. destruct (O.eq_dec v x3).
+      * unfold O.eq in e. subst.
+ apply app_inversion in H1.
+        intuition.
+      right.  apply app_inversion in H1.
+      ex
+       
+      destruct (O.eq_dec x3 v).
+
+
+ destruct o. destruct (G.contains_vertex g v0). destruct H1. destruct x1; inversion H; subst.
+ inversion H.
+  
+  
+
+
+
+  valid_dfs_state s g o ->
+  In (x, Some y) ->
+  
+  
 
 
 (*Let's prove a stronger version of this
